concurrency/JuicyMachineModule.v
@@ -63,9 +63,9 @@ Module THE_JUICY_MACHINE.
   Definition tp_bupd P (tp : jstate) := (exists phi, join_all tp phi) /\
   forall phi, join_all tp phi ->
     forall c : ghost,
-     joins (ghost_of phi) (ghost_fmap (approx (level phi)) (approx (level phi)) c) ->
+     joins (ghost_of phi) (ghost_fmap (approx (level phi)) (approx (level phi)) (Some (initial_world.ext_ghost tt, NoneP) :: c)) ->
      exists b : ghost,
-       joins b (ghost_fmap (approx (level phi)) (approx (level phi)) c) /\
+       joins b (ghost_fmap (approx (level phi)) (approx (level phi)) (Some (initial_world.ext_ghost tt, NoneP) :: c)) /\
        exists phi' tp', tp_update tp phi tp' phi' /\ ghost_of phi' = b /\ P tp'.
 
   Existing Instance JuicyMachineShell.
