concurrency/semax_conc.v
@@ -496,7 +496,7 @@ Program Definition freelock2_spec cs: funspec := mk_funspec
    | (v, sh, sh', Q, R) =>
      PROP (writable_share sh)
      LOCAL (temp _lock v)
-     SEP (weak_positive_mpred R && weak_rec_inv sh' v Q R && emp; lock_inv sh v R)
+     SEP (weak_exclusive_mpred R && weak_rec_inv sh' v Q R && emp; lock_inv sh v R)
    end)
   (fun _ x =>
    match x with
@@ -515,26 +515,26 @@ Next Obligation.
   apply (nonexpansive2_super_non_expansive
    (fun Q R => (PROP (writable_share sh)
      LOCAL (temp _lock v)
-     SEP (weak_positive_mpred R && weak_rec_inv sh' v Q R && emp; lock_inv sh v R)) rho));
+     SEP (weak_exclusive_mpred R && weak_rec_inv sh' v Q R && emp; lock_inv sh v R)) rho));
   [ clear Q R; intros Q;
     apply (PROP_LOCAL_SEP_nonexpansive
             ((fun _ => writable_share sh) :: nil)
             (temp _lock v :: nil)
-            ((fun R => weak_positive_mpred R && weak_rec_inv sh' v Q R && emp)%logic :: (fun R => lock_inv sh v R) :: nil))
+            ((fun R => weak_exclusive_mpred R && weak_rec_inv sh' v Q R && emp)%logic :: (fun R => lock_inv sh v R) :: nil))
   | clear Q R; intros R;
     apply (PROP_LOCAL_SEP_nonexpansive
             ((fun _ => writable_share sh) :: nil)
             (temp _lock v :: nil)
-            ((fun Q => weak_positive_mpred R && weak_rec_inv sh' v Q R && emp)%logic :: (fun _ => lock_inv sh v R) :: nil))];
+            ((fun Q => weak_exclusive_mpred R && weak_rec_inv sh' v Q R && emp)%logic :: (fun _ => lock_inv sh v R) :: nil))];
   repeat apply Forall_cons; try apply Forall_nil.
   + apply const_nonexpansive.
-  + apply (conj_nonexpansive (fun R => weak_positive_mpred R && weak_rec_inv sh' v Q R)%logic); [apply (conj_nonexpansive weak_positive_mpred) |].
-    - apply positive_mpred_nonexpansive.
+  + apply (conj_nonexpansive (fun R => weak_exclusive_mpred R && weak_rec_inv sh' v Q R)%logic); [apply (conj_nonexpansive weak_exclusive_mpred) |].
+    - apply exclusive_mpred_nonexpansive.
     - apply rec_inv1_nonexpansive.
     - apply const_nonexpansive.
   + apply nonexpansive_lock_inv.
   + apply const_nonexpansive.
-  + apply (conj_nonexpansive (fun Q => weak_positive_mpred R && weak_rec_inv sh' v Q R)%logic); [apply (conj_nonexpansive (fun _ => weak_positive_mpred R)) |].
+  + apply (conj_nonexpansive (fun Q => weak_exclusive_mpred R && weak_rec_inv sh' v Q R)%logic); [apply (conj_nonexpansive (fun _ => weak_exclusive_mpred R)) |].
     - apply const_nonexpansive.
     - apply rec_inv2_nonexpansive.
     - apply const_nonexpansive.
